Base execution on ReactorType rather than Reactor

src/ReactorModel/Determinism/Dependency.lean
@@ -2,31 +2,29 @@ import ReactorModel.Execution
 
 open Classical ReactorType
 
-theorem ReactorType.Wellformed.rcn_state_deps_local {rtr : Reactor}
+theorem ReactorType.Proper.rcn_state_deps_local [Proper α] {rtr : α}
     (hc₁ : rtr[.rtr][c₁] = some con₁) (hc₂ : rtr[.rtr][c₂] = some con₂) 
-    (hr₁ : con₁.rcns i₁ = some rcn₁) (hr₂ : con₂.rcns i₂ = some rcn₂)
+    (hr₁ : rcns con₁ i₁ = some rcn₁) (hr₂ : rcns con₂ i₂ = some rcn₂)
     (hd₁ : ⟨.stv, j⟩ ∈ rcn₁.deps k₁) (hd₂ : ⟨.stv, j⟩ ∈ rcn₂.deps k₂) : c₁ = c₂ := by
-  have hv₁ := rtr.wellformed.valid_deps hc₁ hr₁ hd₁
-  have hv₂ := rtr.wellformed.valid_deps hc₂ hr₂ hd₂
+  have hv₁ := wellformed rtr |>.valid_deps hc₁ hr₁ hd₁
+  have hv₂ := wellformed rtr |>.valid_deps hc₂ hr₂ hd₂
   cases hk₁ : rcn₁.kind <;> cases hk₂ : rcn₂.kind <;> simp [hk₁, hk₂] at hv₁ hv₂
   all_goals 
     cases hv₁; cases hv₂
     exact Indexable.mem_cpt?_rtr_eq hc₁ hc₂ (cpt := .stv) ‹_› ‹_› 
 
 -- This proposition states that `rcn₂` does not depend on `rcn₁`.
-abbrev NotDependent (rtr : Reactor) (rcn₁ rcn₂ : ID) : Prop :=
+abbrev NotDependent [Indexable α] (rtr : α) (rcn₁ rcn₂ : ID) : Prop :=
   ¬(rcn₁ <[rtr] rcn₂)
 
 notation:50 rcn₁ " ≮[" rtr "] " rcn₂ => NotDependent rtr rcn₁ rcn₂
 
-variable {rtr : Reactor}
-
-theorem NotDependent.deps_disjoint {d} (hi : i₁ ≮[rtr] i₂) (h₁ : rtr[.rcn][i₁] = some rcn₁)
-    (h₂ : rtr[.rcn][i₂] = some rcn₂) (h : d ∈ rcn₁.deps .out) (hs : d.cpt ≠ .stv) : 
-    d ∉ rcn₂.deps .in :=
+theorem NotDependent.deps_disjoint [Indexable α] {rtr : α} {d} (hi : i₁ ≮[rtr] i₂) 
+    (h₁ : rtr[.rcn][i₁] = some rcn₁) (h₂ : rtr[.rcn][i₂] = some rcn₂) (h : d ∈ rcn₁.deps .out) 
+    (hs : d.cpt ≠ .stv) : d ∉ rcn₂.deps .in :=
   byContradiction fun hd => absurd (Dependency.depOverlap h₁ h₂ h (not_not.mp hd) hs) hi
 
-structure Independent (rtr : Reactor) (rcn₁ rcn₂ : ID) : Prop where
+structure Independent [Indexable α] (rtr : α) (rcn₁ rcn₂ : ID) : Prop where
   not_eq : rcn₁ ≠ rcn₂  
   left   : rcn₁ ≮[rtr] rcn₂
   right  : rcn₂ ≮[rtr] rcn₁
@@ -35,13 +33,13 @@ namespace Independent
 
 notation:50 rcn₁ " ≮[" rtr "]≯ " rcn₂ => Independent rtr rcn₁ rcn₂
 
-theorem symm (hi : i₁ ≮[rtr]≯ i₂) : i₂ ≮[rtr]≯ i₁ where
+theorem symm [Indexable α] {rtr : α} (hi : i₁ ≮[rtr]≯ i₂) : i₂ ≮[rtr]≯ i₁ where
   not_eq := hi.not_eq.symm
   left   := hi.right
   right  := hi.left
 
-theorem ne_con_state_mem_rcn₁_deps_not_mem_rcn₂_deps
-    (hc : rtr[.rtr][c] = some con) (hr₁ : con.rcns i₁ = some rcn₁) (hr₂ : con.rcns i₂ = some rcn₂) 
+theorem ne_con_state_mem_rcn₁_deps_not_mem_rcn₂_deps [Proper α] {rtr : α}
+    (hc : rtr[.rtr][c] = some con) (hr₁ : rcns con i₁ = some rcn₁) (hr₂ : rcns con i₂ = some rcn₂) 
     (hd : ⟨.stv, j⟩ ∈ rcn₁.deps .out) (hi : i₁ ≮[rtr]≯ i₂) (hs : .stv j v ∈ rcn₁ i) : 
     ⟨.stv, j⟩ ∉ rcn₂.deps k := by
   by_contra hd'
@@ -56,14 +54,14 @@ theorem ne_con_state_mem_rcn₁_deps_not_mem_rcn₂_deps
     have := Dependency.mutNorm hc ‹_› hr₁ hm₂ (by simp_all [Reaction.Mutates])
     contradiction
   all_goals
-    cases rtr.wellformed.hazards_prio hc hr₁ hr₂ hn hd hd' (.inl rfl)
+    cases Proper.wellformed rtr |>.hazards_prio hc hr₁ hr₂ hn hd hd' (.inl rfl)
     all_goals
       case _ hp =>
       have := Dependency.prio hc ‹_› ‹_› (by simp [*]) hp   
       contradiction
     
 open Indexable in
-theorem state_mem_rcn₁_deps_not_mem_rcn₂_deps 
+theorem state_mem_rcn₁_deps_not_mem_rcn₂_deps [Proper α] {rtr : α}
     (h₁ : rtr[.rcn][i₁] = some rcn₁) (h₂ : rtr[.rcn][i₂] = some rcn₂)
     (hi : i₁ ≮[rtr]≯ i₂) (hs : .stv j v ∈ rcn₁.body i) : ⟨.stv, j⟩ ∉ rcn₂.deps k := by
   have ⟨c₁, _, hc₁, hr₁⟩ := obj?_split h₁ 
@@ -73,7 +71,7 @@ theorem state_mem_rcn₁_deps_not_mem_rcn₂_deps
   by_cases hc : c₁ = c₂
   case neg => 
     by_contra hd₂
-    exact absurd (ReactorType.Wellformed.rcn_state_deps_local hc₁ hc₂ hr₁ hr₂ hd₁ hd₂) hc
+    exact absurd (ReactorType.Proper.rcn_state_deps_local hc₁ hc₂ hr₁ hr₂ hd₁ hd₂) hc
   case pos => 
     injection hc₂ ▸ hc ▸ hc₁ with h
     exact ne_con_state_mem_rcn₁_deps_not_mem_rcn₂_deps hc₁ hr₁ (h ▸ hr₂) hd₁ hi hs
@@ -81,10 +79,12 @@ theorem state_mem_rcn₁_deps_not_mem_rcn₂_deps
 end Independent
 
 -- Reaction `rcn` is maximal wrt. `rcns` if `rcn` does not depend on any reaction in `rcns`.
-def Minimal (rtr : Reactor) (rcns : List ID) (rcn : ID) : Prop :=
+def Minimal [Indexable α] (rtr : α) (rcns : List ID) (rcn : ID) : Prop :=
   ∀ i ∈ rcns, i ≮[rtr] rcn
 
 namespace Minimal
+
+variable [Indexable α] {rtr rtr₁ rtr₂ : α}
 
 notation:50 rcns " ≮[" rtr "] " rcn => Minimal rtr rcns rcn
 
