src/ReactorModel/Execution/State.lean
@@ -1,90 +1,95 @@
 import ReactorModel.Execution.Reactor
 
 noncomputable section
-open Classical
+open Classical ReactorType Updatable Indexable
 
 namespace Execution
 
 @[ext]
-structure State where
-  rtr : Reactor
+structure State (α) [ReactorType.Indexable α] where
+  rtr : α 
   tag : Time.Tag
   progress : Set ID
 
+variable [ReactorType.Indexable α]
+
 namespace State
 
-class Nontrivial (s : State) : Prop where
+class Nontrivial (s : State α) : Prop where
   nontrivial : s.rtr[.rcn].Nonempty
 
-def Closed (s : State) : Prop := 
+def Closed (s : State α) : Prop := 
   s.progress = s.rtr[.rcn].ids
 
-theorem Closed.progress_Nonempty [n : Nontrivial s] (h : Closed s) : s.progress.Nonempty := by
+theorem Closed.progress_Nonempty {s : State α} [n : Nontrivial s] (h : Closed s) : 
+    s.progress.Nonempty := by
   simp_all [Closed, ←Partial.Nonempty.iff_ids_nonempty]
   exact Nontrivial.nontrivial
 
-structure Allows (s : State) (rcn : ID) : Prop where
+structure Allows (s : State α) (rcn : ID) : Prop where
   mem         : rcn ∈ s.rtr[.rcn] 
-  deps        : s.rtr.dependencies rcn ⊆ s.progress
+  deps        : dependencies s.rtr rcn ⊆ s.progress
   unprocessed : rcn ∉ s.progress
 
-theorem Allows.acyclic {s : State} (a : s.Allows rcn) : ¬(rcn <[s.rtr] rcn) :=
+theorem Allows.acyclic {s : State α} (a : s.Allows rcn) : ¬(rcn <[s.rtr] rcn) :=
   fun hc => absurd (a.deps hc) a.unprocessed
 
-def input (s : State) (rcn : ID) : Reaction.Input where
+def input (s : State α) (rcn : ID) : Reaction.Input where
   val cpt := s.rtr[.rcn][rcn] |>.elim ∅ (restriction · cpt)
   tag := s.tag
 where 
   restriction (rcn : Reaction) (cpt : Reactor.Component.Valued) := 
     s.rtr[cpt].restrict { i | ⟨cpt, i⟩ ∈ rcn.deps .in }
 
-def output (s : State) (rcn : ID) : List Change := 
+def output (s : State α) (rcn : ID) : List Change := 
   s.rtr[.rcn][rcn] |>.elim [] (· $ s.input rcn)
 
-inductive Triggers (s : State) (i : ID) : Prop
+inductive Triggers (s : State α) (i : ID) : Prop
   | intro (mem : s.rtr[.rcn][i] = some rcn) (triggers : rcn.TriggersOn (s.input i))
 
 -- TODO: Is this being used?
-theorem Triggers.progress_agnostic 
+theorem Triggers.progress_agnostic {s₁ s₂ : State α}
     (h : Triggers s₁ i) (hr : s₁.rtr = s₂.rtr) (ht : s₁.tag = s₂.tag) : Triggers s₂ i :=
   sorry
 
-def exec (s : State) (rcn : ID) : State :=
-  { s with rtr := s.rtr.apply' (s.output rcn) }
+def exec (s : State α) (rcn : ID) : State α :=
+  { s with rtr := apply' s.rtr (s.output rcn) }
 
-def record [DecidableEq ID] (s : State) (rcn : ID) : State := 
+def record [DecidableEq ID] (s : State α) (rcn : ID) : State α := 
   { s with progress := s.progress.insert rcn }
 
-theorem record_preserves_rtr (s : State) (rcn : ID) : (s.record rcn).rtr = s.rtr := 
+theorem record_preserves_rtr (s : State α) (rcn : ID) : (s.record rcn).rtr = s.rtr := 
   rfl
 
-theorem record_preserves_tag (s : State) (rcn : ID) : (s.record rcn).tag = s.tag := 
+theorem record_preserves_tag (s : State α) (rcn : ID) : (s.record rcn).tag = s.tag := 
   rfl
 
-theorem mem_record_progress_iff (s : State) (rcn₁ rcn₂ : ID) : 
+theorem mem_record_progress_iff (s : State α) (rcn₁ rcn₂ : ID) : 
     rcn₁ ∈ (s.record rcn₂).progress ↔ (rcn₁ = rcn₂ ∨ rcn₁ ∈ s.progress) := by
   simp [record, Set.insert]
 
-def record' [DecidableEq ID] (s : State) (rcns : List ID) : State := 
+def record' [DecidableEq ID] (s : State α) (rcns : List ID) : State α := 
   { s with progress := s.progress ∪ { i | i ∈ rcns } }
 
-theorem record'_perm_eq {s : State} (h : rcns₁ ~ rcns₂) : s.record' rcns₁ = s.record' rcns₂ := by
+theorem record'_perm_eq {s : State α} (h : rcns₁ ~ rcns₂) : s.record' rcns₁ = s.record' rcns₂ := by
   simp [record', h.mem_iff]
   
-theorem mem_record'_progress_iff (s : State) (rcns : List ID) (i : ID) :
+theorem mem_record'_progress_iff (s : State α) (rcns : List ID) (i : ID) :
     i ∈ (s.record' rcns).progress ↔ (i ∈ s.progress ∨ i ∈ rcns) := by
   simp [record']
 
-structure NextTag (s : State) (next : Time.Tag) : Prop where
-  mem : next ∈ s.rtr.scheduledTags
+structure NextTag (s : State α) (next : Time.Tag) : Prop where
+  mem : next ∈ scheduledTags s.rtr
   bound : s.tag < next
-  least : ∀ g ∈ s.rtr.scheduledTags, (s.tag < g) → (next ≤ g)    
+  least : ∀ g ∈ scheduledTags s.rtr, (s.tag < g) → (next ≤ g)    
 
-theorem NextTag.deterministic (n₁ : NextTag s g₁) (n₂ : NextTag s g₂) : g₁ = g₂ :=
+theorem NextTag.deterministic {s : State α} (n₁ : NextTag s g₁) (n₂ : NextTag s g₂) : g₁ = g₂ :=
   sorry
 
-inductive Advance : State → State → Prop 
+inductive Advance : State α → State α → Prop 
   | mk : (NextTag s next) → Advance s { s with tag := next, progress := ∅ }
+
+variable {s₁ s₂ : State α} 
 
 theorem Advance.progress_empty : (Advance s₁ s₂) → s₂.progress = ∅
   | mk .. => rfl
