src/ReactorModel/Execution/Trace.lean
@@ -2,11 +2,15 @@ import ReactorModel.Execution.State
 
 open Classical
 
+variable [ReactorType.Indexable α]
+
 namespace Execution
 namespace Instantaneous
 namespace Step
 
-inductive Skip : State → State → Type  
+variable {s₁ s₂ : State α}
+
+inductive Skip : State α → State α → Type  
   | mk : (s.Allows rcn) → (¬s.Triggers rcn) → Skip s (s.record rcn)
 
 notation s₁:max " ⇓ₛ " s₂:max => Skip s₁ s₂
@@ -20,7 +24,7 @@ def Skip.allows_rcn : (e : s₁ ⇓ₛ s₂) → s₁.Allows e.rcn
 def Skip.not_triggers : (e : s₁ ⇓ₛ s₂) → ¬s₁.Triggers e.rcn
   | mk _ h => h
 
-inductive Exec : State → State → Type  
+inductive Exec : State α → State α → Type  
   | mk : (s.Allows rcn) → (s.Triggers rcn) → Exec s (s.exec rcn |>.record rcn)
 
 notation s₁:max " ⇓ₑ " s₂:max => Exec s₁ s₂
@@ -31,7 +35,7 @@ def Exec.rcn : (s₁ ⇓ₑ s₂) → ID
 def Exec.allows_rcn : (e : s₁ ⇓ₑ s₂) → s₁.Allows e.rcn
   | mk h .. => h
 
-inductive _root_.Execution.Instantaneous.Step (s₁ s₂ : State)
+inductive _root_.Execution.Instantaneous.Step (s₁ s₂ : State α)
   | skip (e : Skip s₁ s₂)
   | exec (e : Exec s₁ s₂)
 
@@ -47,36 +51,36 @@ end Step
 
 -- TODO?: Once all else is settled, return this to being only transitive but not reflexive.
 --        Then you can remove the `fresh` condiction on `ClosedExecution`.
-inductive Execution : State → State → Type
+inductive Execution : State α → State α → Type
   | refl : Execution s s
   | trans : (s₁ ⇓ᵢ s₂) → (Execution s₂ s₃) → Execution s₁ s₃
 
 notation s₁:max " ⇓ᵢ* " s₂:max => Execution s₁ s₂
 
-def Execution.rcns : (s₁ ⇓ᵢ* s₂) → List ID
+def Execution.rcns {s₁ s₂ : State α} : (s₁ ⇓ᵢ* s₂) → List ID
   | refl => []
   | trans hd tl => hd.rcn :: tl.rcns
 
-structure ClosedExecution (s₁ s₂ : State) where  
+structure ClosedExecution (s₁ s₂ : State α) where  
   exec   : s₁ ⇓ᵢ* s₂
   fresh  : s₁.progress = ∅ 
   closed : s₂.Closed
   
 notation s₁:max " ⇓| " s₂:max => ClosedExecution s₁ s₂
 
-abbrev ClosedExecution.rcns (e : s₁ ⇓| s₂) : List ID :=
+abbrev ClosedExecution.rcns {s₁ s₂ : State α} (e : s₁ ⇓| s₂) : List ID :=
   e.exec.rcns
 
 end Instantaneous
 
 -- Note: We don't clear the ports here.
-structure AdvanceTag (s₁ s₂ : State) where
+structure AdvanceTag (s₁ s₂ : State α) where
   closed : s₁.Closed 
   advance : s₁.Advance s₂
 
 notation s₁:max " ⇓- " s₂:max => AdvanceTag s₁ s₂
 
-inductive Step (s₁ s₂ : State)
+inductive Step (s₁ s₂ : State α)
   | close (h : s₁ ⇓| s₂)
   | advance (h : s₁ ⇓- s₂)
 
@@ -86,7 +90,7 @@ end Execution
 
 open Execution
 
-inductive Execution : State → State → Type
+inductive Execution : State α → State α → Type
   | refl : Execution s s
   | step : (s₁ ⇓ s₂) → (Execution s₂ s₃) → Execution s₁ s₃
 
