src/ReactorModel/Determinism/State.lean
@@ -1,22 +1,25 @@
 import ReactorModel.Determinism.Dependency
 
-open Classical ReactorType
+open Classical ReactorType Indexable
 
 namespace Execution
 namespace State
 
-theorem exec_preserves_tag (s : State) (rcn : ID) : (s.exec rcn).tag = s.tag :=
+theorem exec_preserves_tag [Indexable α] (s : State α) (rcn : ID) : (s.exec rcn).tag = s.tag :=
   rfl
 
-theorem exec_preserves_progress (s : State) (rcn : ID) : (s.exec rcn).progress = s.progress :=
+theorem exec_preserves_progress [Indexable α] (s : State α) (rcn : ID) : 
+    (s.exec rcn).progress = s.progress :=
   rfl
 
-theorem exec_equiv (s : State) (rcn : ID) : s.rtr ≈ (s.exec rcn).rtr := by
+theorem exec_equiv [Indexable α] (s : State α) (rcn : ID) : s.rtr ≈ (s.exec rcn).rtr := by
   simp [exec]
-  exact Equivalent.symm $ Reactor.apply'_equiv _ _
+  exact Equivalent.symm $ apply'_equiv _ _
 
-theorem target_not_mem_indep_output {s : State} {i} {i₁ i₂ : ID} (h₂ : s.rtr[.rcn][i₂] = some rcn₂) 
-    (hi : i₁ ≮[s.rtr]≯ i₂) (hd : ⟨cpt, i⟩ ∈ rcn₂.deps .in) : 
+variable [Proper α] {s : State α}
+
+theorem target_not_mem_indep_output 
+    (h₂ : s.rtr[.rcn][i₂] = some rcn₂) (hi : i₁ ≮[s.rtr]≯ i₂) (hd : ⟨cpt, i⟩ ∈ rcn₂.deps .in) : 
     (s.output i₁).All₂ (¬·.Targets cpt i) := by
   apply List.all₂_iff_forall.mpr
   intro c hc
@@ -32,15 +35,15 @@ theorem target_not_mem_indep_output {s : State} {i} {i₁ i₂ : ID} (h₂ : s.r
     all_goals 
       exact hi.left.deps_disjoint h₁ h₂ (rcn₁.target_mem_deps hc) $ by simp [Change.Normal.target]
     
-theorem exec_indep_restriction_eq {s : State} (hi : i₁ ≮[s.rtr]≯ i₂) 
-    (h₂ : s.rtr[.rcn][i₂] = some rcn₂) : 
+theorem exec_indep_restriction_eq (hi : i₁ ≮[s.rtr]≯ i₂) (h₂ : s.rtr[.rcn][i₂] = some rcn₂) : 
     input.restriction (s.exec i₁) rcn₂ cpt = input.restriction s rcn₂ cpt := by 
   simp [input.restriction]
   apply Partial.ext_restrict 
   intro _ hd
-  exact Reactor.apply'_preserves_unchanged $ target_not_mem_indep_output h₂ hi hd  
+  exact apply'_preserves_unchanged $ target_not_mem_indep_output h₂ hi hd  
   
-theorem exec_indep_input_eq {s : State} (hi : i₁ ≮[s.rtr]≯ i₂) (h : s.rtr[.rcn][i₂] = some rcn₂)
+theorem exec_indep_input_eq 
+    (hi : i₁ ≮[s.rtr]≯ i₂) (h : s.rtr[.rcn][i₂] = some rcn₂)
     (h' : (s.exec i₁).rtr[.rcn][i₂] = some rcn₂) : (s.exec i₁).input i₂ = s.input i₂ := by 
   simp [input, h, h']
   refine ⟨?_, by simp [exec]⟩
@@ -48,14 +51,13 @@ theorem exec_indep_input_eq {s : State} (hi : i₁ ≮[s.rtr]≯ i₂) (h : s.rt
   injection h' ▸ Equivalent.obj?_rcn_eq (s.exec_equiv i₁) ▸ h with h'
   exact h'.symm ▸ exec_indep_restriction_eq hi h 
     
-theorem exec_indep_output_eq {s : State} (hi : i₁ ≮[s.rtr]≯ i₂) : 
-    (s.exec i₁).output i₂ = s.output i₂ := by 
+theorem exec_indep_output_eq (hi : i₁ ≮[s.rtr]≯ i₂) : (s.exec i₁).output i₂ = s.output i₂ := by 
   simp [output]
   have e := Equivalent.obj?_rcn_eq $ s.exec_equiv i₁
   cases h : s.rtr[.rcn][i₂] <;> simp [e ▸ h]
   simp [exec_indep_input_eq hi h $ e ▸ h]
 
-theorem indep_normal_output_disjoint {s : State} (hi : i₁ ≮[s.rtr]≯ i₂) :
+theorem indep_normal_output_disjoint (hi : i₁ ≮[s.rtr]≯ i₂) :
     List.Disjoint (s.output i₁ |>.filter (·.IsNormal)) (s.output i₂ |>.filter (·.IsNormal)) := by
   cases h₁ : s.rtr[.rcn][i₁] <;> cases h₂ : s.rtr[.rcn][i₂] <;> simp [output, *]
   case some.some rcn₁ rcn₂ =>
@@ -69,18 +71,18 @@ theorem indep_normal_output_disjoint {s : State} (hi : i₁ ≮[s.rtr]≯ i₂) 
       simp [Change.Normal.target] at hc₁ hc₂
       cases hc : c.cpt <;> try cases ‹Kind›
       case stv =>
-        by_cases h : 
-        have ⟨_, _, h₁, ho₁⟩ := Indexable.obj?_split h₁
-        have ⟨_, _, h₂, ho₂⟩ := Indexable.obj?_split h₂
-        
-        have := s.rtr.wellformed.overlap_prio h₁ ho₁ (hc ▸ hc₁)
-        have := s.rtr.wellformed.state_local h₂ ho₂ (hc ▸ hc₂)
+        -- by_cases h : 
+        -- have ⟨_, _, h₁, ho₁⟩ := Indexable.obj?_split h₁
+        -- have ⟨_, _, h₂, ho₂⟩ := Indexable.obj?_split h₂
+        -- 
+        -- have := s.rtr.wellformed.overlap_prio h₁ ho₁ (hc ▸ hc₁)
+        -- have := s.rtr.wellformed.state_local h₂ ho₂ (hc ▸ hc₂)
         sorry -- You've trying to construct a dependency between 
       case act => sorry
       case prt.in => sorry
       case prt.out => sorry
 
-theorem exec_indep_swap {s : State} (hi : rcn₁ ≮[s.rtr]≯ rcn₂) : 
+theorem exec_indep_swap (hi : rcn₁ ≮[s.rtr]≯ rcn₂) : 
     (s.exec rcn₁).exec rcn₂ = (s.exec rcn₂).exec rcn₁ := by 
   ext1
   case tag => apply exec_preserves_tag
@@ -88,7 +90,7 @@ theorem exec_indep_swap {s : State} (hi : rcn₁ ≮[s.rtr]≯ rcn₂) :
   case rtr =>
     conv => lhs; rw [exec, exec_indep_output_eq hi]
     conv => rhs; rw [exec, exec_indep_output_eq hi.symm]
-    apply Reactor.apply'_normal_disjoint_comm $ indep_normal_output_disjoint hi
+    apply apply'_normal_disjoint_comm $ indep_normal_output_disjoint hi
   
 namespace State
 namespace Execution
